Blanc.lean
@@ -1,4 +1,8 @@
 import Blanc.Solvent
 
+namespace Blanc
+
 def main : List String → IO Unit
   | _ => IO.print "Hello World!"
+
+end Blanc
