scripts/AxiomCheck.lean
@@ -1,6 +1,6 @@
 import Blanc.Solvent
 
-#print axioms weth_preserves_solvent
-#print axioms stateTransition_preserves_solvent
-#print axioms chain_preserves_solvent
-#print axioms addBlockToChain_preserves_solvent
+#print axioms Blanc.weth_preserves_solvent
+#print axioms Blanc.stateTransition_preserves_solvent
+#print axioms Blanc.chain_preserves_solvent
+#print axioms Blanc.addBlockToChain_preserves_solvent
